src/program_proof/twophase/wrapper_proof.v
@@ -23,6 +23,9 @@ Section proof.
   Context `{hRG: !refinement_heapG Σ}.
   Existing Instance jrnlG0.
 
+  Notation spec_ext := jrnl_spec_ext.
+  Notation sval := (@val (@spec_ext_op_field spec_ext)).
+
   Implicit Types (N: namespace).
 
   Definition is_twophase_system N γ :=
@@ -30,19 +33,31 @@ Section proof.
 
   Definition val_of_obj (o : obj) := val_of_list ((λ u, LitV (LitByte u)) <$> o).
 
-  Definition jrnl_mapsto_own addr obj : iProp Σ :=
-    ∃ obj', jrnl_mapsto addr 1 obj' ∗ ⌜data_has_obj obj' addr obj⌝.
+  Definition bufObj_to_obj bufObj : obj :=
+    match objData bufObj with
+    | bufBit b => [U8 (if b then 1 else 0)]
+    | bufInode data | bufBlock data => data
+    end.
 
-  Definition jrnl_maps_have_mt_changed (σj1 σj2: jrnl_map) (mt_changed: gmap addr versioned_object) :=
-    dom (gset addr) (jrnlData σj1) = dom (gset addr) (jrnlData σj2) ∧
-    map_Forall (λ addr vobj,
-      match mt_changed !! addr with
-      | Some vobj' =>
-        data_has_obj vobj.1 addr (committed vobj') ∧
-        data_has_obj vobj.2 addr (modified vobj')
-      | None => vobj.1 = vobj.2
-      end
-    ) (map_zip (jrnlData σj1) (jrnlData σj2)).
+  Definition jrnl_mapsto_own a bufObj : iProp Σ :=
+    "Hmapsto" ∷ jrnl_mapsto a 1 (bufObj_to_obj bufObj) ∗
+    "Htok" ∷ jrnl_crash_tok a.
+
+  Global Instance jrnl_mapsto_own_Timeless a bufObj:
+    Timeless (jrnl_mapsto_own a bufObj).
+  Proof. refine _. Qed.
+
+  Global Instance jrnl_mapsto_own_Discretizable a bufObj:
+    Discretizable (jrnl_mapsto_own a bufObj).
+  Proof. refine _. Qed.
+
+  Definition jrnl_maps_kinds_valid γ (σj1 σj2: jrnl_map) :=
+    jrnlKinds σj1 = γ.(buftxn_txn_names).(txn_kinds) ∧
+    jrnlKinds σj2 = γ.(buftxn_txn_names).(txn_kinds).
+
+  Definition jrnl_maps_have_mt (mt_changed: gmap addr versioned_object) (σj1 σj2: jrnl_map) :=
+    bufObj_to_obj <$> (committed <$> mt_changed) = jrnlData σj1 ∧
+    bufObj_to_obj <$> (modified <$> mt_changed) = jrnlData σj2.
 
   Definition is_twophase_pre l (γ γ' : buftxn_names) dinit (objs_dom: gset addr) : iProp Σ :=
     ∃ (txnl locksl : loc) ghs,
@@ -51,33 +66,42 @@ Section proof.
       "#Histxn_system" ∷ is_txn_system Nbuftxn γ ∗
       "#Histxn" ∷ is_txn txnl γ.(buftxn_txn_names) dinit ∗
       "#HlockMap" ∷ is_lockMap locksl ghs (set_map addr2flat objs_dom)
-        (twophase_linv_flat 0 jrnl_mapsto_own γ) ∗
+        (twophase_linv_flat 0 jrnl_mapsto_own γ γ') ∗
+      "#Hspec_ctx" ∷ spec_ctx ∗
+      "#Hspec_crash_ctx" ∷ spec_crash_ctx jrnl_crash_ctx ∗
+      "#Hjrnl_open" ∷ jrnl_open ∗
+      "#Hjrnl_kinds_lb" ∷ jrnl_kinds_lb γ.(buftxn_txn_names).(txn_kinds) ∗
       "#Htxn_cinv" ∷ txn_cinv Nbuftxn γ γ' ∗
-      "%Hvalids" ∷ ⌜set_Forall valid_addr objs_dom⌝.
+      "%Haddrs_valid" ∷ ⌜set_Forall valid_addr objs_dom⌝.
 
-  Definition is_twophase_started l γ dinit objs_dom j K e1 e2 : iProp Σ :=
-    ∃ σj1 σj2 mt_changed ls,
+  Definition is_twophase_started l γ γ' dinit objs_dom j K e1 e2 : iProp Σ :=
+    ∃ σj1 σj2 mt_changed (ls: sval),
       (* mark: do we need is_twophase_pre in here too? *)
       "Hj" ∷ j ⤇ K (Atomically ls e1) ∗
       "Htwophase" ∷ is_twophase_raw
-        l γ dinit 0 jrnl_mapsto_own objs_dom mt_changed ∗
-      "%Halways_steps" ∷ ⌜ always_steps e1 σj1 e2 σj2 ⌝ ∗
-      "%Hmt_changed" ∷ ⌜ jrnl_maps_have_mt_changed σj1 σj2 mt_changed ⌝.
+        l γ γ' dinit 0 jrnl_mapsto_own objs_dom mt_changed ∗
+      "#Hspec_ctx" ∷ spec_ctx ∗
+      "#Hspec_crash_ctx" ∷ spec_crash_ctx jrnl_crash_ctx ∗
+      "#Hjrnl_open" ∷ jrnl_open ∗
+      "#Hjrnl_kinds_lb" ∷ jrnl_kinds_lb γ.(buftxn_txn_names).(txn_kinds) ∗
+      "%Halways_steps" ∷ ⌜always_steps e1 σj1 e2 σj2⌝ ∗
+      "%Hjrnl_maps_kinds" ∷ ⌜jrnl_maps_kinds_valid γ σj1 σj2⌝ ∗
+      "%Hjrnl_maps_mt" ∷ ⌜jrnl_maps_have_mt mt_changed σj1 σj2⌝.
 
-  Definition is_twophase_releasable l γ (objs_dom: gset addr) : iProp Σ :=
+  Definition is_twophase_releasable l γ γ' (objs_dom: gset addr) : iProp Σ :=
     ∃ locks_held mt_changed σj1 σj2,
       (* mark: do we need is_twophase_pre in here too? *)
       "Hlocks" ∷ is_twophase_locks
-        l γ 0 jrnl_mapsto_own (set_map addr2flat objs_dom) locks_held ∗
+        l γ γ' 0 jrnl_mapsto_own (set_map addr2flat objs_dom) locks_held ∗
       "Hlinvs" ∷ ([∗ list] flat_a ∈ locks_held, (
-        "Hlinv" ∷ twophase_linv_flat 0 jrnl_mapsto_own γ flat_a
+        "Hlinv" ∷ twophase_linv_flat 0 jrnl_mapsto_own γ γ' flat_a
       )) ∗
       "%Hlocks_held" ∷ ⌜
         set_map addr2flat (dom (gset addr) mt_changed) =
         (list_to_set locks_held: gset u64)
       ⌝ ∗
-      "%Hmt_changed" ∷ ⌜ jrnl_maps_have_mt_changed σj1 σj2 mt_changed ⌝ ∗
-      "%Hvalids" ∷ ⌜set_Forall valid_addr objs_dom⌝.
+      "%Hjrnl_maps_kinds" ∷ ⌜jrnl_maps_kinds_valid γ σj1 σj2⌝ ∗
+      "%Hjrnl_maps_mt" ∷ ⌜jrnl_maps_have_mt mt_changed σj1 σj2⌝.
 
   Theorem wpc_Init N (d: loc) γ dinit logm mt k :
     N ## invN →
@@ -88,7 +112,11 @@ Section proof.
       "Hmapstos" ∷ ([∗ map] a ↦ obj ∈ mt,
         "Hdurable_mapsto" ∷ durable_mapsto_own γ a obj ∗
         "Hjrnl_mapsto" ∷ jrnl_mapsto_own a obj
-      )
+      ) ∗
+      "#Hspec_ctx" ∷ spec_ctx ∗
+      "#Hspec_crash_ctx" ∷ spec_crash_ctx jrnl_crash_ctx ∗
+      "#Hjrnl_open" ∷ jrnl_open ∗
+      "#Hjrnl_kinds_lb" ∷ jrnl_kinds_lb γ.(buftxn_txn_names).(txn_kinds)
     }}}
       Init #d @ k; ⊤
     {{{
@@ -101,8 +129,8 @@ Section proof.
       (⌜ γ' = γ ⌝ ∨ txn_cinv Nbuftxn γ γ')
     }}}.
   Proof.
-    iIntros (HinvN HwalN Hvalids Φ Φc) "(?&?) HΦ".
-    iNamed.
+    iIntros (HinvN HwalN Hvalids Φ Φc) "Hpre HΦ".
+    iNamed "Hpre".
     wpc_call.
     {
       iExists _, _.
@@ -147,7 +175,7 @@ Section proof.
     }
     iNamed.
     wp_apply (
-      wp_MkLockMap _ (twophase_linv_flat 0 jrnl_mapsto_own γ)
+      wp_MkLockMap _ (twophase_linv_flat 0 jrnl_mapsto_own γ γ')
       with "[Hlinvs]"
     ).
     {
@@ -177,107 +205,249 @@ Section proof.
     assumption.
   Qed.
 
-  Theorem wp_TwoPhase__Begin' N prel γ γ' dinit objs_dom j K ls e1 :
+  Lemma map_Forall_exists {A B} `{Countable K} (m: gmap K A) P :
+    map_Forall (λ a x, ∃ y, P a x y) m →
+    ∃ (m': gmap K B),
+      dom (gset K) m = dom (gset K) m' ∧
+      map_Forall (λ a xy, P a xy.1 xy.2) (map_zip m m').
+  Proof.
+    induction m as [|a x m_sub] using map_ind.
+    {
+      intros _.
+      exists ∅.
+      split; first by rewrite !dom_empty_L //.
+      intros k x Hacc.
+      rewrite map_zip_lookup_none_1 in Hacc; last by auto.
+      inversion Hacc.
+    }
+    intros Hex.
+    apply map_Forall_insert_1_1 in Hex as Hex1.
+    apply map_Forall_insert_1_2 in Hex as Hex2; last by assumption.
+    apply IHm in Hex2.
+    destruct Hex1 as [y Hex1].
+    destruct Hex2 as [m'_sub [Hdoms Hm'_sub]].
+    exists (<[a:=y]>m'_sub).
+    split; first by rewrite !dom_insert_L -Hdoms //.
+    rewrite map_zip_insert.
+    apply map_Forall_insert_2; assumption.
+  Qed.
+
+  Lemma map_Forall_zip_snd {A B} `{Countable K} (m1: gmap K A) (m2: gmap K B) P :
+    dom (gset K) m2 ⊆ dom (gset K) m1 →
+    map_Forall (λ a xy, P a xy.2) (map_zip m1 m2) →
+    map_Forall P m2.
+  Proof.
+    intros Hdoms Hforall k y Hacc.
+    apply mk_is_Some in Hacc as Hacc'.
+    apply elem_of_dom in Hacc'.
+    apply (iffLR (elem_of_subseteq _ _) Hdoms k) in Hacc'.
+    apply elem_of_dom in Hacc'.
+    destruct Hacc' as [x Hacc'].
+    pose proof (map_zip_lookup_some _ _ _ _ _ Hacc' Hacc) as Hacc_zip.
+    apply Hforall in Hacc_zip.
+    assumption.
+  Qed.
+
+  Theorem wp_TwoPhase__Begin' N prel γ γ' dinit objs_dom j K (ls: sval) e1 :
     {{{
       "Htwophase" ∷ is_twophase_pre prel γ γ' dinit objs_dom ∗
       "Hatom" ∷ j ⤇ K (Atomically ls e1)
     }}}
       Begin #prel
     {{{ tphl, RET #tphl;
-        is_twophase_started tphl γ dinit objs_dom j K e1 e1 }}}.
+        is_twophase_started tphl γ γ' dinit objs_dom j K e1 e1 }}}.
   Proof.
-    iIntros (Φ) "(?&Hatom) HΦ".
-    iNamed.
+    iIntros (Φ) "Hpre HΦ".
+    iNamed "Hpre".
     iNamed "Htwophase".
     wp_apply (wp_TwoPhase__Begin_raw with "[$]"); first by assumption.
     iIntros (?) "?".
     iNamed.
+
     iApply "HΦ".
-    iExists (∅, ∅), (∅, ∅), _, _.
-    iFrame.
+    iExists (∅, _), (∅, _), _, _.
+    iFrame "∗ #".
     iPureIntro.
     split.
-    - apply always_steps_refl.
-      rewrite /wf_jrnl /offsets_aligned /sizes_correct dom_empty_L /=.
-      set_solver.
-    - rewrite /jrnl_maps_have_mt_changed /=.
-      split; first by reflexivity.
-      rewrite map_zip_empty_r.
-      apply map_Forall_empty.
+    2: {
+      split; first by rewrite /jrnl_maps_kinds_valid //.
+      rewrite /jrnl_maps_have_mt !fmap_empty //.
+    }
+    apply always_steps_refl.
+    rewrite /wf_jrnl /offsets_aligned dom_empty_L //.
   Qed.
 
-  Theorem wp_TwoPhase__CommitNoRelease' l γ dinit objs_dom j K e1 v :
-    {{{ is_twophase_started l γ dinit objs_dom j K e1 (SOMEV v) }}}
+  Theorem wp_TwoPhase__CommitNoRelease' l γ γ' dinit objs_dom j K {HCTX: LanguageCtx K} e1 v :
+    {{{ is_twophase_started l γ γ' dinit objs_dom j K e1 (SOMEV v) }}}
       TwoPhase__CommitNoRelease #l
     {{{ (ok:bool), RET #ok;
-        if ok then
-          is_twophase_releasable l γ objs_dom ∗
-          j ⤇ K (SOMEV v)
-        else
-          is_twophase_started l γ dinit objs_dom j K e1 (SOMEV v)
+        "Htwophase" ∷ is_twophase_releasable l γ γ' objs_dom ∗
+        "Hj" ∷ (
+          if ok then
+            j ⤇ K (SOMEV v)
+          else
+            (* j ⤇ K NONEV *)
+            ∃ ls e1, j ⤇ K (Atomically ls e1)
+        )
     }}}.
-  Proof. Admitted.
+  Proof.
+    iIntros (Φ) "Htwophase HΦ".
+    iNamed "Htwophase".
+    iDestruct (is_twophase_raw_get_valid with "Htwophase") as "%Hvalids".
+    unshelve (wp_apply (
+      wp_TwoPhase__CommitNoRelease_raw
+      _ _ _ _ _ _ _ _
+      (j ⤇ K (SOMEV v))%I
+      (j ⤇ K (Atomically ls e1))%I
+      with "[$Htwophase Hj]"
+    )).
+    1-2: refine _.
+    {
+      iSplit.
+      - iIntros "!> ?".
+        iNamed.
+        iAssert (
+          [∗ map] a ↦ o ∈ jrnlData σj1,
+            "Hmapsto" ∷ jrnl_mapsto a 1 o ∗
+            "Htok" ∷ jrnl_crash_tok a
+        )%I with "[Hcommitted]" as "Hcommitted".
+        {
+          destruct Hjrnl_maps_mt as [<- _].
+          rewrite !big_sepM_fmap //.
+        }
+        iDestruct (big_sepM_sep with "Hcommitted") as "[Hmapstos Htoks]".
+        destruct Hjrnl_maps_kinds as [<- _].
+        iDestruct (
+          ghost_step_jrnl_atomically_crash
+          with "Hspec_crash_ctx Hmapstos Htoks Hjrnl_kinds_lb Hjrnl_open Hj"
+        ) as "> [Hmapstos Htoks]"; [eassumption|set_solver|].
+        iModIntro.
+        iApply big_sepM_sep.
+        destruct Hjrnl_maps_mt as [<- <-].
+        rewrite !big_sepM_fmap.
+        iFrame.
+      - iIntros "!> ?".
+        iNamed.
+        iAssert (
+          [∗ map] a ↦ o ∈ jrnlData σj1,
+            "Hmapsto" ∷ jrnl_mapsto a 1 o ∗
+            "Htok" ∷ jrnl_crash_tok a
+        )%I with "[Hcommitted]" as "Hcommitted".
+        {
+          destruct Hjrnl_maps_mt as [<- _].
+          rewrite !big_sepM_fmap //.
+        }
+        iDestruct (big_sepM_sep with "Hcommitted") as "[Hmapstos Htoks]".
+        destruct Hjrnl_maps_kinds as [<- _].
+        iSplit.
+        2: {
+          iFrame.
+          iApply big_sepM_sep.
+          destruct Hjrnl_maps_mt as [<- _].
+          rewrite !big_sepM_fmap.
+          iFrame.
+        }
+        iDestruct (
+          ghost_step_jrnl_atomically
+          with "Hspec_ctx Hmapstos Hjrnl_kinds_lb Hjrnl_open Hj"
+        ) as "> [Hj Hmapstos]"; [eassumption|set_solver|].
+        iModIntro.
+        iFrame.
+        destruct Hjrnl_maps_mt as [<- <-].
+        rewrite !big_sepM_fmap.
+        iApply big_sepM_sep.
+        iFrame.
+    }
+    iIntros (??) "Hpost".
+    iNamed "Hpost".
+    iApply "HΦ".
+    iSplitL "Hlocks Hlinvs".
+    {
+      iExists _, _, _, _.
+      iDestruct (is_twophase_locks_get_pures with "Hlocks")
+        as "#Hlocks_pures".
+      iNamed "Hlocks_pures".
+      iFrame "∗ %".
+      rewrite -big_sepS_list_to_set; last by assumption.
+      rewrite -Hlocks_held.
+      iApply big_sepS_set_map; last by iFrame.
 
-  Theorem twophase_started_abort l γ dinit objs_dom j K e1 e2 :
-    is_twophase_started l γ dinit objs_dom j K e1 e2 -∗
-    |NC={⊤}=> is_twophase_releasable l γ objs_dom ∗
+      intros a1 a2 Hacc1 Hacc2 Heq.
+      apply elem_of_dom in Hacc1.
+      apply elem_of_dom in Hacc2.
+      destruct Hacc1 as [vo1 Hacc1].
+      destruct Hacc2 as [vo2 Hacc2].
+      apply Hvalids in Hacc1.
+      apply Hvalids in Hacc2.
+      rewrite /mapsto_valid in Hacc1.
+      rewrite /mapsto_valid in Hacc2.
+      apply addr2flat_eq; intuition.
+    }
+    destruct ok; first by iFrame.
+    iExists _, _.
+    iFrame.
+  Qed.
+
+  Theorem twophase_started_abort l γ γ' dinit objs_dom j K e1 e2 :
+    is_twophase_started l γ γ' dinit objs_dom j K e1 e2 -∗
+    |NC={⊤}=> is_twophase_releasable l γ γ' objs_dom ∗
               j ⤇ K NONEV.
   Proof. Admitted.
 
-  Theorem wp_TwoPhase__ReleaseAll' l γ objs_dom :
-    {{{ is_twophase_releasable l γ objs_dom }}}
+  Theorem wp_TwoPhase__ReleaseAll' l γ γ' objs_dom :
+    {{{ is_twophase_releasable l γ γ' objs_dom }}}
       TwoPhase__ReleaseAll #l
     {{{ RET #(); True }}}.
   Proof. Admitted.
 
-  Theorem wp_TwoPhase__ReadBuf' l γ dinit objs_dom j K0 K
+  Theorem wp_TwoPhase__ReadBuf' l γ γ' dinit objs_dom j K0 K
           {Hctx: LanguageCtx'
             (ext := @spec_ext_op_field _)
             (ffi := (spec_ffi_model_field))
             (ffi_semantics := (spec_ext_semantics_field))
             K} e1 a sz :
     {{{
-      is_twophase_started l γ dinit objs_dom j K0 e1
+      is_twophase_started l γ γ' dinit objs_dom j K0 e1
         (K (ExternalOp (ext := @spec_ext_op_field jrnl_spec_ext)
           ReadBufOp (PairV (addr2val' a) #sz)))
     }}}
       TwoPhase__ReadBuf' #l (addr2val a, #sz)
     {{{ v, RET (val_of_obj v);
-        is_twophase_started l γ dinit objs_dom j K0 e1
+        is_twophase_started l γ γ' dinit objs_dom j K0 e1
           (K (val_of_obj' v))
     }}}.
   Proof. Admitted.
 
-  Theorem wp_TwoPhase__OverWrite' l γ dinit objs_dom j K0 K
+  Theorem wp_TwoPhase__OverWrite' l γ γ' dinit objs_dom j K0 K
           {Hctx: LanguageCtx'
             (ext := @spec_ext_op_field _)
             (ffi := (spec_ffi_model_field))
             (ffi_semantics := (spec_ext_semantics_field))
             K}  e1 a ov :
     {{{
-      is_twophase_started l γ dinit objs_dom j K0
+      is_twophase_started l γ γ' dinit objs_dom j K0
         e1
         (K (ExternalOp (ext := @spec_ext_op_field jrnl_spec_ext)
           OverWriteOp (PairV (addr2val' a) (val_of_obj' ov)))) }}}
       TwoPhase__OverWrite' #l (addr2val a, val_of_obj ov)
     {{{ RET #();
-        is_twophase_started l γ dinit objs_dom j K0
+        is_twophase_started l γ γ' dinit objs_dom j K0
                             e1 (K #())
     }}}.
   Proof. Admitted.
 
-  Lemma twophase_started_step_puredet l γ dinit objs_dom j K0 K
+  Lemma twophase_started_step_puredet l γ γ' dinit objs_dom j K0 K
         `{Hctx: LanguageCtx'
           (ext := @spec_ext_op_field _)
           (ffi := (spec_ffi_model_field))
           (ffi_semantics := (spec_ext_semantics_field))
           K} e0 e1 e2:
     (∀ σ, prim_step' e1 σ [] e2 σ []) →
-    is_twophase_started l γ dinit objs_dom j K0 e0 (K e1) -∗
-    is_twophase_started l γ dinit objs_dom j K0 e0 (K e2).
+    is_twophase_started l γ γ' dinit objs_dom j K0 e0 (K e1) -∗
+    is_twophase_started l γ γ' dinit objs_dom j K0 e0 (K e2).
   Proof. Admitted.
 
-  Lemma twophase_started_ub_det l γ dinit objs_dom E j K0 K
+  Lemma twophase_started_ub_det l γ γ' dinit objs_dom E j K0 K
         `{Hctx: LanguageCtx'
           (ext := @spec_ext_op_field _)
           (ffi := (spec_ffi_model_field))
@@ -285,7 +455,7 @@ Section proof.
           K} e0 e :
     nclose sN ⊆ E →
     (∀ s, stuck' e s) →
-    is_twophase_started l γ dinit objs_dom j K0 e0 (K e)
+    is_twophase_started l γ γ' dinit objs_dom j K0 e0 (K e)
     -∗ |NC={E}=> False.
   Proof. Admitted.
 
